---
title: Example Problems
date: 2023-09-07
tags:
  - modules
  - group-algebras
  - examples
  - incomplete
---
*These problems were sourced from UW Madison MATH 542 Fall 2023 in-class material*
## 1. Show that $0\cdot m = 0$ for all $m\in M$. Use this to show that $(-1)\cdot m = -m$.
*Proof.* We see that $$\begin{align*}0\cdot m &= (0 + 0)\cdot m,\\
&=0\cdot m + 0\cdot m.\end{align*}$$
Applying left or right cancellation by $0\cdot m$ yields $0 \cdot m = 0$. Using this result, $$\begin{align*}0 &= 0\cdot m,\\
&= (1 + (-1))\cdot m,\\
&=1\cdot m + (-1)\cdot m,\\
&= m + (-1)\cdot m.\end{align*}$$
So $(-1)\cdot m$ is the inverse of $m$ and consequently $(-1)\cdot m = -m$ as desired. 

## 2.

## 3.

## 4.
